src/theories/Reflection/FM.v
@@ -8,6 +8,15 @@ Require Import MetaCoq.Template.All.
 Require Import MirrorSolve.Reflection.Core.
 Set Universe Polymorphism.
 
+Require Import MirrorSolve.HLists.
+
+MetaCoq Quote Definition c_True := True.
+MetaCoq Quote Definition c_False := False.
+MetaCoq Quote Definition c_eq := @eq.
+MetaCoq Quote Definition c_not := @not.
+MetaCoq Quote Definition c_or := @or.
+MetaCoq Quote Definition c_and := @and.
+
 Section ReflectFM.
   Variable (s: signature).
   Variable (m: model s).
@@ -18,23 +27,16 @@ Section ReflectFM.
   Variable (sort_eq_dec: EquivDec.EqDec (sig_sorts s) eq).
 
   Equations mk_var (c: ctx s) (n: nat) : option ({srt & var s c srt}) by struct n := 
-    mk_var (CSnoc c' srt) 0 := Some (existT _ srt (VHere _ _ srt));
-    mk_var (CSnoc c' srt) (S n') := 
+    mk_var (Snoc _ c' srt) 0 := Some (existT _ srt (VHere _ _ srt));
+    mk_var (Snoc _ c' srt) (S n') := 
       let nxt := mk_var c' n' in 
       match nxt with 
       | Some v =>
-        let (srt', v') := v in 
-        Some (existT _ srt' (VThere _ _ _ _ v'))
+        let (ty', v') := v in 
+        Some (existT _ ty' (VThere _ _ _ _ v'))
       | None => None
       end;
-    mk_var CEmp _ := None.
-
-  MetaCoq Quote Definition c_True := True.
-  MetaCoq Quote Definition c_False := False.
-  MetaCoq Quote Definition c_eq := @eq.
-  MetaCoq Quote Definition c_not := @not.
-  MetaCoq Quote Definition c_or := @or.
-  MetaCoq Quote Definition c_and := @and.
+    mk_var SLNil _ := None.
 
   Fixpoint reflect_t2tm' (c: ctx s) (acc: nat) (t: term) : option ({srt & tm s c srt}) :=  
     match t with 
@@ -113,7 +115,7 @@ Section ReflectFM.
             let srt := reflect_ind2srt i in 
             match srt with 
             | Some srt => 
-              let c' := CSnoc _ c srt in
+              let c' := Snoc _ c srt in
               let inner := reflect_t2fm c' acc pst in 
               match inner with 
               | Some fm => Some (FForall _ fm)
@@ -136,15 +138,139 @@ Section ReflectFM.
   MetaCoq Quote Definition test_1 := (False -> True).
   MetaCoq Quote Definition test_2 := (True = False -> False).
   MetaCoq Quote Definition test_3 := (~ ~ False).
-  MetaCoq Quote Definition test_4 := (False).
+  MetaCoq Quote Definition test_4 := (False /\ True).
   MetaCoq Quote Definition test_5 := (forall (x: unit), True).
   MetaCoq Quote Definition test_6 := (forall (x: unit), True \/ False \/ ~ True).
 
-  Eval vm_compute in reflect_t2fm c test_1.
-  Eval vm_compute in reflect_t2fm c test_2. 
-  Eval vm_compute in reflect_t2fm c test_3.
-  Eval vm_compute in reflect_t2fm c test_4.
-  Eval vm_compute in reflect_t2fm c test_5.
-  Eval vm_compute in reflect_t2fm c test_6. *)
+  Eval vm_compute in reflect_t2fm c 0 test_1.
+  Eval vm_compute in reflect_t2fm c 0 test_2. 
+  Eval vm_compute in reflect_t2fm c 0 test_3.
+  Eval vm_compute in reflect_t2fm c 0 test_4.
+  Eval vm_compute in reflect_t2fm c 0 test_5.
+  Eval vm_compute in reflect_t2fm c 0 test_6. *)
 End ReflectFM.
     
+
+
+
+Section ParseFM.
+  Variable (Ty: Type).
+  Variable (interp_ty: Ty -> Type).
+
+  Variable (ty_eq_dec: EquivDec.EqDec Ty eq).
+
+  Notation res_ty := (option ({ty & interp_ty ty})).
+  Notation env_ty := (snoc_list ({ty & interp_ty ty})).
+
+  Variable (parse_t2tm : term -> list res_ty -> res_ty).
+  Variable (parse_ind : inductive -> option Ty).
+
+  Fixpoint parse_var (env: env_ty) (n: nat) : res_ty :=
+    match env, n with 
+    | Snoc _ x, 0 => Some x
+    | Snoc env' _, S n' => parse_var env' n'
+    | SLNil, _ => None
+    end.
+
+  Fixpoint parse_t2tm' (env: env_ty) (acc: nat) (t: term) : res_ty :=  
+    match t with 
+    | tRel n => parse_var env (n - acc)
+    | tApp f es => parse_t2tm t (map (parse_t2tm' env acc) es)
+    | _ => parse_t2tm t []
+    end.
+
+  Definition ret (p: Prop) : option (env_ty -> option Prop) := Some (fun _ => Some p).
+
+  Obligation Tactic := intros.
+  Equations parse_t2fm (env: env_ty) (anon_acc: nat) (t: term) : option Prop by struct t := 
+    parse_t2fm env acc t := 
+      if eq_term t c_True then Some True else 
+      if eq_term t c_False then Some False else
+      match t with
+      | tApp f es => 
+        if eq_term f c_eq then 
+          match es with 
+          | _ :: tl :: tr :: _ => 
+            match parse_t2tm' env acc tl, parse_t2tm' env acc tr with 
+            | Some l, Some r => 
+              let (tl, el) := l in 
+              let (tr, er) := r in 
+                match ty_eq_dec tl tr with 
+                | left HEq => 
+                  Some (el = (eq_rect_r _ er HEq))
+                | _ => None
+                end
+            | _, _ => None
+            end
+          | _ => None
+          end
+        else if eq_term f c_or then 
+          match es with 
+          | tl :: tr :: _ => 
+            match parse_t2fm env acc tl, parse_t2fm env acc tr with 
+            | Some l, Some r => Some (l \/ r)
+            | _, _ => None
+            end
+          | _ => None
+          end
+        else if eq_term f c_and then 
+          match es with 
+          | tl :: tr :: _ => 
+            match parse_t2fm env acc tl, parse_t2fm env acc tr with 
+            | Some l, Some r => Some (l /\ r)
+            | _, _ => None
+            end
+          | _ => None
+          end
+        else if eq_term f c_not then 
+          match es with 
+          | x :: _ => 
+            match parse_t2fm env acc x with 
+            | Some x' => Some (~ x')
+            | None => None
+            end
+          | _ => None
+          end
+        else
+          None
+      | tProd ba_name pre pst => 
+        match ba_name.(binder_name) with 
+        | nAnon =>
+          match parse_t2fm env acc pre, parse_t2fm env (S acc) pst with 
+          | Some el, Some er => Some (el -> er)
+          | _, _ => None
+          end
+        | nNamed _ =>
+          match pre with 
+          | tInd i _ => 
+            let ty := parse_ind i in 
+            match ty with
+            | Some ty' => Some (
+              forall x: interp_ty ty', 
+              exists p',
+              let env' := Snoc _ env (existT _ ty' x) in
+                  parse_t2fm env' acc pst = Some p' /\
+                  p'
+              )
+            | None => None
+            end
+          | _ => None
+          end
+        end
+      | _ => None
+      end.
+
+  (* MetaCoq Quote Definition test_1 := (False -> True).
+  MetaCoq Quote Definition test_2 := (True = False -> False).
+  MetaCoq Quote Definition test_3 := (~ ~ False).
+  MetaCoq Quote Definition test_4 := (False /\ True).
+  MetaCoq Quote Definition test_5 := (forall (x: unit), x = tt).
+  MetaCoq Quote Definition test_6 := (forall (x: unit), True \/ False \/ ~ True).
+
+  Eval vm_compute in parse_t2fm (SLNil _)  0 test_1.
+  Eval vm_compute in parse_t2fm (SLNil _)  0 test_2. 
+  Eval vm_compute in parse_t2fm (SLNil _)  0 test_3.
+  Eval vm_compute in parse_t2fm (SLNil _)  0 test_4.
+  Eval vm_compute in parse_t2fm (SLNil _)  0 test_5.
+  Eval vm_compute in parse_t2fm (SLNil _)  0 test_6. *)
+End ParseFM.
