src/theories/Reflection/Core.v
@@ -1,5 +1,7 @@
 
 Require Export MetaCoq.Template.All.
+(* Require Import MetaCoq.Checker.All. *)
+
 Require Import MetaCoq.Template.Checker.
 
 Definition eq_term (l r: term) : bool := 
